Cleaned up xor and card

src/cnf/cnf.lean
@@ -20,7 +20,7 @@ import data.nat.basic
 universe u
 
 -- Represents the parametric type of the variable stored in the literal
-variables {V : Type*} [decidable_eq V] [inhabited V]
+variables {V : Type*}
 
 /- Conjunctive normal form is a list of clauses joined by logical ANDs -/
 def cnf (V : Type*) := list (clause V)
@@ -28,8 +28,7 @@ def cnf (V : Type*) := list (clause V)
 -- Note that the above definition allows for duplication of clauses (and
 -- permutations of clauses), whereas a set definition would not (assuming a
 -- set definition of clauses as well). However, lists allow for computable 
--- functions to be defined on them, which is important for proving that
--- encoding methods, which are computable, are equisatisfiable
+-- functions to be defined on them.
 
 namespace cnf
 
@@ -41,18 +40,18 @@ open finset
 
 /-! # Instance properties -/
 
-instance : inhabited (cnf V) := ⟨[arbitrary (clause V)]⟩
+instance [inhabited V] : inhabited (cnf V) := ⟨[arbitrary (clause V)]⟩
 instance : has_mem (clause V) (cnf V) := ⟨list.mem⟩
 instance : has_emptyc (cnf V) := ⟨list.nil⟩
-instance : has_union (cnf V) := ⟨list.union⟩
-instance : has_inter (cnf V) := ⟨list.inter⟩
+instance [decidable_eq V] : has_union (cnf V) := ⟨list.union⟩
+instance [decidable_eq V] : has_inter (cnf V) := ⟨list.inter⟩
 instance : has_singleton (clause V) (cnf V) := ⟨λ c, [c]⟩ 
-instance : has_insert (clause V) (cnf V) := ⟨list.insert⟩
+instance [decidable_eq V] : has_insert (clause V) (cnf V) := ⟨list.insert⟩
 instance : has_append (cnf V) := ⟨list.append⟩
 instance : has_subset (cnf V) := ⟨list.subset⟩
 instance [has_repr V] : has_repr (cnf V) := ⟨list.repr⟩
 
-instance (c : clause V) (f : cnf V) : decidable (c ∈ f) :=
+instance [decidable_eq V] (c : clause V) (f : cnf V) : decidable (c ∈ f) :=
 begin
   induction f with cl cls ih,
   { exact decidable.false },
@@ -64,29 +63,26 @@ begin
 end
 
 /-! ### Evaluation under assignment -/
+section eval
 
--- Note: The below implementation works as well as a countp/filter, too
-/- The clauses of the CNF are joined by conjunctions, so for the evaluation
-   of a formula to be true, all clauses within must evaluate to true -/
+variables {τ : assignment V} {c : clause V} {f : cnf V}
+
 protected def eval (τ : assignment V) (f : cnf V) : bool :=
   f.foldr (λ c b, b && (clause.eval τ c)) tt
 
-@[simp] theorem eval_nil {τ : assignment V} : cnf.eval τ [] = tt := rfl
+@[simp] theorem eval_nil : cnf.eval τ [] = tt := rfl
 
-@[simp] theorem eval_singleton {τ : assignment V} {c : clause V} : 
-  cnf.eval τ [c] = clause.eval τ c :=
+@[simp] theorem eval_singleton : cnf.eval τ [c] = c.eval τ :=
 by simp only [cnf.eval, foldr, tt_band]
 
-theorem eval_cons {τ : assignment V} {c : clause V} {f : cnf V} : 
-  cnf.eval τ (c :: f) = (clause.eval τ c && cnf.eval τ f) :=
+@[simp] theorem eval_cons : cnf.eval τ (c :: f) = c.eval τ && f.eval τ :=
 by simp only [cnf.eval, foldr, bool.band_comm]
 
-theorem eval_ff_cons_of_eval_ff {τ : assignment V} {f : cnf V} (c : clause V) :
-  cnf.eval τ f = ff → cnf.eval τ (c :: f) = ff :=
+theorem eval_ff_cons_of_eval_ff (c : clause V) : f.eval τ = ff → cnf.eval τ (c :: f) = ff :=
 assume h, by rw [eval_cons, h, band_ff]
 
 theorem eval_append (τ : assignment V) (f₁ f₂ : cnf V) : 
-  cnf.eval τ (f₁ ++ f₂) = cnf.eval τ f₁ && cnf.eval τ f₂ :=
+  cnf.eval τ (f₁ ++ f₂) = f₁.eval τ && f₂.eval τ :=
 begin
   unfold cnf.eval,
   rw foldr_append,
@@ -95,71 +91,79 @@ begin
   { rw band_tt }
 end
 
-theorem eval_tt_iff_forall_clause_eval_tt {τ : assignment V} {f : cnf V} :
-  cnf.eval τ f = tt ↔ ∀ c ∈ f, clause.eval τ c = tt :=
+theorem eval_tt_iff_forall_clause_eval_tt : f.eval τ = tt ↔ ∀ (c : clause V), c ∈ f → c.eval τ = tt :=
 begin
-  split,
-  { induction f with c cs ih,
-    { intros _ c hc, exact absurd hc (not_mem_nil _) },
-    { simp [eval_cons],
-      intros hc hcs,
-      exact and.intro hc (ih hcs) } },
-  { induction f with c cs ih,
-    { rw eval_nil, tautology },
-    { simp [eval_cons],
-      intros hc hcs,
-      exact and.intro hc (ih hcs) } }
+  induction f with c cs ih,
+  { simp only [eval_nil, eq_self_iff_true, not_mem_nil, is_empty.forall_iff, implies_true_iff] },
+  { simp only [ih, eval_cons, band_eq_true_eq_eq_tt_and_eq_tt, mem_cons_iff, forall_eq_or_imp] }
 end
 
-theorem eval_ff_iff_exists_clause_eval_ff {τ : assignment V} {f : cnf V} :
-  cnf.eval τ f = ff ↔ ∃ c ∈ f, clause.eval τ c = ff :=
+theorem eval_ff_iff_exists_clause_eval_ff : f.eval τ = ff ↔ ∃ c, c ∈ f ∧ clause.eval τ c = ff :=
 begin
-  split,
-  { induction f with c cs ih,
-    { rw eval_nil, contradiction },
-    { simp [eval_cons],
-      rintros (hc | hcs),
-      { use [c, hc] },
-      { rcases ih hcs with ⟨cl, hcl₁, hcl₂⟩,
-        use [cl, or.inr hcl₁, hcl₂] } } },
-  { induction f with c cs ih,
-    { rintros ⟨cl, hcl, _⟩, exact absurd hcl (not_mem_nil _) },
-    { rintros ⟨cl, hcl, heval⟩,
-      rcases eq_or_mem_of_mem_cons hcl with rfl | h,
-      { rw [eval_cons, heval, ff_band] },
-      { exact eval_ff_cons_of_eval_ff c (ih ⟨cl, h, heval⟩) } } }
+  induction f with c cs ih,
+  { simp only [eval_nil, not_mem_nil, false_and, exists_false] },
+  { simp only [eval_cons, band_eq_false_eq_eq_ff_or_eq_ff, mem_cons_iff],
+    split,
+    { rintros (h | h),
+      { use [c, or.inl rfl, h] },
+      { rcases ih.mp h with ⟨c₂, hc, he⟩,
+        use [c₂, mem_cons_of_mem c hc, he] } },
+    { rintros ⟨c₂, (rfl | hc), he⟩,
+      { exact or.inl he },
+      { exact or.inr (ih.mpr ⟨c₂, hc, he⟩) } } }
 end
 
-theorem ne_nil_of_eval_ff {τ : assignment V} {f : cnf V} :
-  f.eval τ = ff → f ≠ [] :=
-begin
-  intro h,
-  rcases eval_ff_iff_exists_clause_eval_ff.mp h with ⟨cl, hcl, _⟩,
-  exact ne_nil_of_mem hcl
-end
+end eval
 
 def satisfiable (f : cnf V) := ∃ τ, f.eval τ = tt
 
-theorem satisfiable_of_eval_tt (f : cnf V) (τ : assignment V) :
-  f.eval τ = tt → satisfiable f :=
+theorem satisfiable_of_eval_tt (f : cnf V) (τ : assignment V) : f.eval τ = tt → satisfiable f :=
 assume h, exists.intro τ h
 
 /-! ### Counting -/
+section counting
 
-/- Counts the number of clauses which evaluate to true under some assignment -/
-protected def count_tt (τ : assignment V) (f : cnf V) : nat :=
-  f.countp (λ c, clause.eval τ c = tt)
+variables (τ : assignment V) (c : clause V) (f f₁ f₂ : cnf V)
 
-/- Counts the number of clauses which evaluate to false under some assignment -/
-protected def count_ff (τ : assignment V) (f : cnf V) : nat :=
-  f.countp (λ c, clause.eval τ c = ff)
+protected def count_tt : nat := f.countp (λ c, clause.eval τ c = tt)
+protected def count_ff : nat := f.countp (λ c, clause.eval τ c = ff)
 
-@[simp] theorem count_tt_nil (τ : assignment V) : cnf.count_tt τ [] = 0 := rfl
-@[simp] theorem count_ff_nil (τ : assignment V) : cnf.count_ff τ [] = 0 := rfl
+@[simp] theorem count_tt_nil : cnf.count_tt τ [] = 0 := rfl
+@[simp] theorem count_ff_nil : cnf.count_ff τ [] = 0 := rfl
+
+@[simp] theorem count_tt_singleton : cnf.count_tt τ [c] = cond (c.eval τ) 1 0 :=
+by cases h : (c.eval τ); simp [h, cnf.count_tt]
+
+@[simp] theorem count_ff_singleton : cnf.count_ff τ [c] = cond (c.eval τ) 0 1 :=
+by cases h : (c.eval τ); simp [h, cnf.count_ff]
+
+@[simp] theorem count_tt_cons : cnf.count_tt τ (c :: f) = cond (c.eval τ) (1 + f.count_tt τ) (f.count_tt τ) :=
+by cases h : (c.eval τ); simp [h, cnf.count_tt, add_comm]
+
+@[simp] theorem count_ff_cons : cnf.count_ff τ (c :: f) = cond (c.eval τ) (f.count_ff τ) (1 + f.count_ff τ) :=
+by cases h : (c.eval τ); simp [h, cnf.count_ff, add_comm]
+
+theorem count_tt_append : cnf.count_tt τ (f₁ ++ f₂) = cnf.count_tt τ f₁ + cnf.count_tt τ f₂ :=
+begin
+  induction f₁ with c cs ih,
+  { simp only [nil_append, count_tt_nil, zero_add] },
+  { cases h : (c.eval τ); simp [h, ih, add_assoc] }
+end
+
+theorem count_ff_append : cnf.count_ff τ (f₁ ++ f₂) = cnf.count_ff τ f₁ + cnf.count_ff τ f₂ :=
+begin
+  induction f₁ with c cs ih,
+  { simp only [nil_append, count_ff_nil, zero_add] },
+  { cases h : (c.eval τ); simp [h, ih, add_assoc] }
+end
+
+end counting
 
 /-! # vars -/
+section vars
 
--- Extract the variables used in the clauses, as a set
+variables [decidable_eq V] {v : V} {c : clause V} {f f₁ f₂ : cnf V}
+
 protected def vars : cnf V → finset V
 | []        := ∅
 | (c :: cs) := (c.vars) ∪ (vars cs)
@@ -169,6 +173,9 @@ protected def vars : cnf V → finset V
 @[simp] theorem vars_singleton (c : clause V) : cnf.vars [c] = clause.vars c :=
 by { unfold cnf.vars, rw finset.union_empty }
 
+theorem mem_vars_cons_of_mem_vars (c : clause V) : v ∈ f.vars → v ∈ cnf.vars (c :: f) :=
+assume h, finset.mem_union.mpr (or.inr h)
+
 theorem vars_append (f₁ f₂ : cnf V) : cnf.vars (f₁ ++ f₂) = f₁.vars ∪ f₂.vars :=
 begin
   induction f₁ with c cs ih,
@@ -176,12 +183,20 @@ begin
   { simp only [cnf.vars, cons_append c cs f₂, ih, finset.union_assoc] }
 end
 
-theorem mem_vars_cons_of_mem_vars {f : cnf V} {v : V} (c : clause V) :
-  v ∈ f.vars → v ∈ cnf.vars (c :: f) :=
-assume h, finset.mem_union.mpr (or.inr h)
+theorem vars_perm : f₁ ~ f₂ → f₁.vars = f₂.vars :=
+begin
+  intro hp,
+  induction hp with _ _ _ _ IH  x y _  _ _ _ _ _ IH₁ IH₂,
+  { refl },
+  { unfold cnf.vars, rw IH },
+  { unfold cnf.vars,
+    rw [← finset.union_assoc, ← finset.union_assoc, finset.union_comm y.vars x.vars] },
+  { exact eq.trans IH₁ IH₂ }
+end
 
-theorem clause_vars_subset_of_vars_of_mem {f : cnf V} {c : clause V} :
-  c ∈ f → (c.vars) ⊆ f.vars :=
+--theorem vars_perm_strong :
+
+theorem clause_vars_subset_of_vars_of_mem : c ∈ f → c.vars ⊆ f.vars :=
 begin
   induction f with cl cls ih,
   { intro h, exact absurd h (not_mem_nil _) },
@@ -193,8 +208,7 @@ begin
     { exact mem_vars_cons_of_mem_vars cl (ih hc hv) } }
 end
 
-theorem mem_vars_iff_exists_mem_clause_and_mem {f : cnf V} {v : V} :
-  v ∈ f.vars ↔ ∃ (c : clause V), c ∈ f ∧ v ∈ c.vars :=
+theorem mem_vars_iff_exists_mem_clause_and_mem : v ∈ f.vars ↔ ∃ (c : clause V), c ∈ f ∧ v ∈ c.vars :=
 begin
   induction f with cl cls ih,
   { simp only [not_mem_empty, not_mem_nil, exists_false, vars_nil, false_and] },
@@ -208,57 +222,36 @@ begin
       rw cnf.vars,
       rcases eq_or_mem_of_mem_cons hc with (rfl | hc),
       { exact finset.mem_union_left _ hv },
-      { apply finset.mem_union_right,
-        exact ih.mpr ⟨c, hc, hv⟩ } } }
+      { exact finset.mem_union_right _ (ih.mpr ⟨c, hc, hv⟩) } } }
 end
 
-theorem vars_subset_of_subset {f₁ f₂ : cnf V} :
-  f₁ ⊆ f₂ → (cnf.vars f₁) ⊆ (cnf.vars f₂) :=
+theorem vars_subset_of_subset : f₁ ⊆ f₂ → (cnf.vars f₁) ⊆ (cnf.vars f₂) :=
 begin
   intros h v hv,
   rcases cnf.mem_vars_iff_exists_mem_clause_and_mem.mp hv with ⟨c, hf, hvc⟩,
   exact clause_vars_subset_of_vars_of_mem (h hf) hvc
 end
 
+end vars
+
 /-! # Equisatisfiability -/
 
-def equisatisfiable (f₁ f₂ : cnf V) :=
-  (∃ (τ₁ : assignment V), cnf.eval τ₁ f₁ = tt) ↔ 
-   ∃ (τ₂ : assignment V), cnf.eval τ₂ f₂ = tt
+def eqsat (f₁ f₂ : cnf V) := satisfiable f₁ ↔ satisfiable f₂
 
 --notation f₁ ` ≈ ` f₂ := equisatisfiable f₁ f₂
 
-@[simp] theorem equisatisfiable_nil : equisatisfiable ([] : cnf V) [] :=
-⟨λ h, h, λ h, h⟩
+@[refl] theorem eqsat.refl (f : cnf V) : eqsat f f := ⟨id, id⟩
 
-@[refl] theorem equisatisfiable.refl (f : cnf V) : equisatisfiable f f :=
-⟨λ h, h, λ h, h⟩
+@[symm] theorem eqsat.symm (f₁ f₂ : cnf V) : eqsat f₁ f₂ → eqsat f₂ f₁ := λ h, ⟨h.2, h.1⟩
 
-@[symm] theorem equisatisfiable.symm (f₁ f₂ : cnf V) :
-  equisatisfiable f₁ f₂ → equisatisfiable f₂ f₁ :=
-assume h, ⟨h.2, h.1⟩
-
-@[trans] theorem equisatisfiable.trans {f₁ f₂ f₃ : cnf V} :
-  equisatisfiable f₁ f₂ → equisatisfiable f₂ f₃ → equisatisfiable f₁ f₃ :=
-begin
-  rintros ⟨hmp1, hmpr1⟩ ⟨hmp2, hmpr2⟩,
-  split,
-  { intro h, exact hmp2 (hmp1 h) },
-  { intro h, exact hmpr1 (hmpr2 h) }
-end
-
-end cnf
+@[trans] theorem eqsat.trans {f₁ f₂ f₃ : cnf V} : eqsat f₁ f₂ → eqsat f₂ f₃ → eqsat f₁ f₃ :=
+λ h₁ h₂, ⟨λ h, h₂.1 (h₁.1 h), λ h, h₁.2 (h₂.2 h)⟩
 
 /-! # Equivalence on domain theorems -/
 
-namespace assignment
+open assignment
 
-open literal
-open clause
-open cnf
-open list
-
-theorem eval_eq_cnf_of_eqod {τ₁ τ₂ : assignment V} {f : cnf V} :
+theorem eval_eq_of_eqod [decidable_eq V] {τ₁ τ₂ : assignment V} {f : cnf V} :
   (eqod τ₁ τ₂ f.vars) → f.eval τ₁ = f.eval τ₂ :=
 begin
   intro h,
@@ -266,13 +259,12 @@ begin
   { apply eval_ff_iff_exists_clause_eval_ff.mpr,
     rcases eval_ff_iff_exists_clause_eval_ff.mp hev with ⟨c, hc, hff⟩,
     use [c, hc],
-    exact hff ▸ eval_eq_clause_of_eqod 
+    exact hff ▸ clause.eval_eq_of_eqod 
       (eqod_subset (clause_vars_subset_of_vars_of_mem hc) h) },
   { apply eval_tt_iff_forall_clause_eval_tt.mpr,
     intros c hc,
-    have := eval_tt_iff_forall_clause_eval_tt.mp hev c hc,
-    exact this ▸ eval_eq_clause_of_eqod
+    exact (eval_tt_iff_forall_clause_eval_tt.mp hev c hc) ▸ clause.eval_eq_of_eqod
       (eqod_subset (clause_vars_subset_of_vars_of_mem hc) h) }
 end
 
-end assignment
+end cnf
