src/cnf/explode.lean
@@ -17,16 +17,10 @@ import data.nat.pow
 universe u
 
 -- Represents the parametric type of the variable stored in the literal
-variables {V : Type*} [decidable_eq V] [inhabited V]
+variables {V : Type*}
 
-open literal
-open clause
-open list
-open function
-
-/- Sometimes, it is necessary to take a list of variables and produce a list
-   of all possible positive and negative forms of those variables, maintaining
-   the order of the original list. We call this operation, "exploding." -/
+open literal clause
+open list function
 
 namespace explode
 
@@ -34,21 +28,20 @@ variables {v : V} {l : list V} {c : clause V}
 
 /-! # Explode -/
 
+-- Produces a list of all possible polarities on a list of variables, maintaining order
 def explode : list V → list (clause V)
 | []        := [[]]
 | (v :: l) := (explode l).map (cons (Pos v)) ++ (explode l).map (cons (Neg v))
 
 @[simp] theorem explode_nil : explode ([] : list V) = [[]] := rfl
 
-@[simp] theorem explode_singleton (v : V) : explode [v] = [[Pos v], [Neg v]] :=
-by refl
+@[simp] theorem explode_singleton (v : V) : explode [v] = [[Pos v], [Neg v]] := rfl
 
 theorem length_explode (l : list V) : length (explode l) = 2^(length l) :=
 begin
   induction l with v vs ih,
   { refl },
-  { simp only [explode, length_cons, length_append, 
-      length_map, pow_succ, two_mul, ih] }
+  { simp only [explode, length_cons, length_append, length_map, pow_succ, two_mul, ih] }
 end
 
 theorem length_explode_pos (l : list V) : length (explode l) > 0 :=
@@ -60,7 +53,7 @@ exists_mem_of_length_pos (length_explode_pos _)
 theorem length_eq_of_mem_explode : c ∈ explode l → length c = length l :=
 begin
   induction l with v vs ih generalizing c,
-  { rw [explode_nil, mem_singleton], 
+  { rw [explode_nil, mem_singleton],
     rintro rfl, refl },
   { simp only [explode, mem_append, mem_map],
     rintros (⟨c, hc, rfl⟩ | ⟨c, hc, rfl⟩);
@@ -71,8 +64,9 @@ theorem cons_mem_explode_cons_of_mem_explode (lit : literal V) :
   c ∈ explode l → (lit :: c) ∈ explode (lit.var :: l) :=
 assume hc, by { cases lit; simp [explode, literal.var, hc] }
 
-theorem mem_of_mem_explode_of_mem_vars : 
-  c ∈ explode l → v ∈ c.vars → v ∈ l :=
+variable [decidable_eq V]
+
+theorem mem_of_mem_explode_of_mem_vars : c ∈ explode l → v ∈ c.vars → v ∈ l :=
 begin
   induction l with v vs ih generalizing c,
   { rw [explode_nil, mem_singleton],
@@ -81,19 +75,14 @@ begin
     exact absurd hv (finset.not_mem_empty _) },
   { simp only [explode, mem_append, mem_map],
     rintros (⟨a, ha, rfl⟩ | ⟨a, ha, rfl⟩);
-    { intros hv,
-      unfold clause.vars at hv,
-      rw finset.mem_union at hv,
-      rw mem_cons_iff,
-      rcases hv with hv | hv,
-      { unfold var at hv,
-        rw finset.mem_singleton at hv,
+    { rw [clause.vars, finset.mem_union, mem_cons_iff],
+      rintros (hv | hv),
+      { rw [var, finset.mem_singleton] at hv,
         exact or.inl hv },
       { exact or.inr (ih ha hv) } } }
 end
 
-theorem mem_vars_of_mem_explode_of_mem :
-  c ∈ explode l → v ∈ l → v ∈ c.vars :=
+theorem mem_vars_of_mem_explode_of_mem : c ∈ explode l → v ∈ l → v ∈ c.vars :=
 begin
   induction l with v vs ih generalizing c,
   { intros _ hv, exact absurd hv (not_mem_nil v) } ,
@@ -105,32 +94,16 @@ begin
       { exact finset.mem_union.mpr (or.inr (ih ha hv)) } } }
 end
 
--- Corollaries of the above
-theorem not_mem_vars_of_mem_explode_of_not_mem :
-  c ∈ explode l → v ∉ l → v ∉ c.vars :=
-begin
-  intro h,
-  contrapose,
-  simp only [not_not],
-  exact mem_of_mem_explode_of_mem_vars h
-end
+theorem not_mem_vars_of_mem_explode_of_not_mem : c ∈ explode l → v ∉ l → v ∉ c.vars :=
+λ h hv, mt (mem_of_mem_explode_of_mem_vars h) hv
 
-theorem not_mem_of_mem_explode_of_not_mem_vars :
-  c ∈ explode l → v ∉ c.vars → v ∉ l :=
-begin
-  intro h,
-  contrapose,
-  simp only [not_not],
-  exact mem_vars_of_mem_explode_of_mem h
-end
+theorem not_mem_of_mem_explode_of_not_mem_vars : c ∈ explode l → v ∉ c.vars → v ∉ l :=
+λ h hv, mt (mem_vars_of_mem_explode_of_mem h) hv
 
-theorem pos_or_neg_of_mem_explode_of_mem :
-  c ∈ explode l → v ∈ l → Pos v ∈ c ∨ Neg v ∈ c :=
-assume h hv, mem_vars_iff_pos_or_neg_mem_clause.mp 
-  (mem_vars_of_mem_explode_of_mem h hv)
+theorem pos_or_neg_of_mem_explode_of_mem : c ∈ explode l → v ∈ l → Pos v ∈ c ∨ Neg v ∈ c :=
+λ h hv, mem_vars_iff_pos_or_neg_mem_clause.mp (mem_vars_of_mem_explode_of_mem h hv)
 
-theorem pos_and_neg_not_mem_of_mem_explode_of_not_mem :
-  c ∈ explode l → v ∉ l → Pos v ∉ c ∧ Neg v ∉ c :=
+theorem pos_and_neg_not_mem_of_mem_explode_of_not_mem : c ∈ explode l → v ∉ l → Pos v ∉ c ∧ Neg v ∉ c :=
 begin
   intro h,
   contrapose,
@@ -141,57 +114,46 @@ begin
     (mem_vars_iff_pos_or_neg_mem_clause.mpr hv)
 end
 
--- A theorems concerning the variables of input
--- If explode changes type to (fin)set, remove/update theorem
+-- If the variables in a clause match the input to explode, then it's in explode
 theorem map_var_eq_iff_mem_explode : c.map var = l ↔ c ∈ explode l :=
 begin
-  split,
-  { induction l with v vs ih generalizing c,
-    { simp only [explode_nil, imp_self, map_eq_nil, mem_singleton] },
+  induction l with v vs ih generalizing c,
+  { simp only [map_eq_nil, explode_nil, mem_singleton] },
+  { split,
     { intro h,
       rcases exists_cons_of_map_cons h with ⟨l, ls, rfl, hl, hls⟩,
-      rcases pos_or_neg_of_var_eq_nat hl with rfl | rfl,
-      { simp [explode], left, use [ls, ih hls] },
-      { simp [explode], right, use [ls, ih hls] } } },
-  { induction l with v vs ih generalizing c,
-    { simp only [explode_nil, imp_self, map_eq_nil, mem_singleton] },
+      cases l; simp only [explode, mem_append, mem_map],
+      { rw var at hl, subst hl, left, use [ls, ih.mp hls] },
+      { rw var at hl, subst hl, right, use [ls, ih.mp hls] } },
     { simp only [explode, mem_map, mem_append],
       rintros (⟨a, ha, rfl⟩ | ⟨a, ha, rfl⟩);
-      { simp only [ih ha, var, map, eq_self_iff_true, and_self] } } }
+      { simp only [ih.mpr ha, var, map, eq_self_iff_true, and_self] } } }
 end
 
 /-! # nodup properties of explode -/
--- Note: These are not necessary if nodup becomes a (fin)set
 
 theorem explode_nodup (l : list V) : nodup (explode l) :=
 begin
   induction l with v vs ih,
   { rw explode_nil, exact nodup_singleton nil },
-  { simp only [explode, nodup_cons, nodup_append],
-    simp only [(nodup_map_iff (cons_injective)).mpr ih, true_and],
+  { simp only [explode, nodup_cons, nodup_append, (nodup_map_iff (cons_injective)).mpr ih, true_and],
     intros x hxp hxn,
-    rcases mem_map.mp hxp with ⟨c, _, hcx⟩,
-    rcases mem_map.mp hxn with ⟨d, _, rfl⟩,
-    have := (head_eq_of_cons_eq hcx).symm,
+    rcases mem_map.mp hxp with ⟨c, _, rfl⟩,
+    rcases mem_map.mp hxn with ⟨d, _, h⟩,
+    have := head_eq_of_cons_eq h,
     contradiction }
 end
 
--- TODO Use simp to reduce?
 theorem nodup_of_nodup_of_mem (h : nodup l) : c ∈ explode l → nodup c :=
 begin
   induction l with n ns ih generalizing c,
   { rw [explode_nil, mem_singleton], rintro rfl, exact nodup_nil },
-  { intro hc,
-    simp only [explode, mem_append, mem_map] at hc,
-    rcases hc with ⟨a, ha, rfl⟩ | ⟨a, ha, rfl⟩,
-    { rw nodup_cons,
-      have := (nodup_cons.mp h).1,
-      have := pos_and_neg_not_mem_of_mem_explode_of_not_mem ha this,
-      exact ⟨this.1, ih (nodup_cons.mp h).2 ha⟩ },
-    { rw nodup_cons,
-      have := (nodup_cons.mp h).1,
-      have := pos_and_neg_not_mem_of_mem_explode_of_not_mem ha this,
-      exact ⟨this.2, ih (nodup_cons.mp h).2 ha⟩ } }
+  { simp only [explode, mem_append, mem_map],
+    rintro (⟨a, ha, rfl⟩ | ⟨a, ha, rfl⟩);
+    rw nodup_cons;
+    have := pos_and_neg_not_mem_of_mem_explode_of_not_mem ha ((nodup_cons.mp h).1),
+    { exact ⟨this.1, ih (nodup_cons.mp h).2 ha⟩ },
+    { exact ⟨this.2, ih (nodup_cons.mp h).2 ha⟩ } }
 end
 
 theorem xor_pos_neg_mem_clause_of_nodup_of_mem_explode_of_mem (h : nodup l) :
@@ -202,8 +164,7 @@ begin
   { simp only [explode, mem_append, mem_map],
     rintros (⟨a, ha, rfl⟩ | ⟨a, ha, rfl⟩) hc;
     { rcases eq_or_mem_of_mem_cons hc with (rfl | hv),
-      { simp [pos_and_neg_not_mem_of_mem_explode_of_not_mem ha 
-            (nodup_cons.mp h).1] },
+      { simp [pos_and_neg_not_mem_of_mem_explode_of_not_mem ha (nodup_cons.mp h).1] },
       { rcases ih (nodup_cons.mp h).2 ha hv with ⟨hp, hn⟩ | ⟨hp, hn⟩;
         { simp [hp, hn, ne_of_mem_of_not_mem hv (nodup_cons.mp h).1] } } } }
 end
